\documentclass[12pt,a4paper]{article}
\usepackage{solutions-en}
\usepackage{float}

\title{Homework of 10.12\\Differential equations and dynamic systems.\\Solutions.}
\author{Глеб Минаев @ 204 (20.Б04-мкн)}
\date{}

\begin{document}
    \maketitle

    \begin{problem}{257}
        \begin{gather*}
            y'^2 - 2xy' = 8x^2\\
            y'^2 - 2xy' - 8x^2 = 0\\
            (y' - 4x)(y' + 2x) = 0\\
            \left[\begin{aligned}
                &y' = 4x\\
                &y' = -2x
            \end{aligned}\right.\\
            \left[\begin{aligned}
                &y = 2x^2 + C\\
                &y = -x^2 + C
            \end{aligned}\right.
        \end{gather*}
        So $2x^2 + C$ and $-x^2 + C$ are the only types of solutions of the equation.

        Singular solution are are solutions of equation
        \begin{gather*}
            2y' - 2x = 0\\
            y' = x.
        \end{gather*}
        No solution of previous equation satisfy the new equation. Hence there is no singular solutions.
    \end{problem}

    \begin{problem}{269}
        \begin{gather*}
            x = y' \sqrt{y'^2 + 1}
        \end{gather*}
        Let $p := y'$. Then $dy = p dx$. So
        \begin{gather*}
            x = p \sqrt{p^2 + 1}\\
            y = \int dy = \int pdx = px - \int x dp = p^2 \sqrt{p^2 + 1} - \int p\sqrt{p^2 + 1} dp\\
            = p^2 \sqrt{p^2 + 1} - \frac{1}{3} (p^2 + 1) \sqrt{p^2 + 1} + C = \sqrt{p^2 + 1} \frac{1}{3} (2p^2 - 1) + C
        \end{gather*}
    \end{problem}

    \begin{problem}{289}
        \begin{gather*}
            y = 2xy' - 4y'^3
        \end{gather*}
        Let $p := y'$. Then $dy = p dx$. So
        \begin{gather*}
            y = 2xp - 4p^3\\
            pdx = dy = 2xdp + 2pdx - 12p^2dp\\
            0 = 2x + px'_p - 12p^2\\
            \frac{d}{dp}(p^2x) = 2px + p^2 x'_p = 12p^3 = \frac{d}{dp}(3p^4)\\
            p^2 x = 3 p^4 + C\\
            x = 3p^2 + \frac{C}{p^2}\\
            y = 2xp - 4p^3 = 6p^3 + \frac{2C}{p} - 4p^3 = 2p^3 + \frac{2C}{p}.
        \end{gather*}
    \end{problem}

    \begin{problem}{293}
        \begin{gather*}
            xy' - y = \ln(y')
        \end{gather*}
        Let $p := y'$. Then $dy = pdx$. So
        \begin{gather*}
            xp - y = \ln(p)\\
            pdx + xdp - pdx = \frac{dp}{p}\\
            xdp = \frac{dp}{p}\\
            x = \frac{1}{p}\\
            y = xp - \ln(p) = 1 - \ln(p)
        \end{gather*}
    \end{problem}

    \begin{problem}{421}
        \begin{gather*}
            x^2 y'' = y'^2.
        \end{gather*}
        Let $p := y'$. Then
        \[x^2 p' = p^2\]
        $x = e^t$, $p = e^t z(t)$. Then $p' = 2 z + z'$. So
        \begin{gather*}
            e^{2t} (2 z + z') = e^{2t} z^2\\
            2z + z' = z^2\\
            \frac{2}{z} - \left(\frac{1}{z}\right)' = 1\\
            e^{-2t}\left(\frac{1}{z}\right)' + \frac{(e^{-2t})'}{z} = -e^{-2t}\\
            \left(\frac{e^{-2t}}{z}\right)' = -e^{-2t}\\
            \frac{e^{-2t}}{z} = \frac{1}{2}e^{-2t} + C\\
            z = \frac{e^{-2t}}{\frac{1}{2}e^{-2t} + C} = \frac{1}{\frac{1}{2} + C e^{2t}} = \frac{2}{C e^{2t} + 1}
        \end{gather*}
        \begin{gather*}
            p = \frac{2 e^t}{C e^{2t} + 1} = \frac{2x}{Cx^2 + 1}\\
            y = \int \frac{2xdx}{Cx^2 + 1} = \frac{\ln(Cx^2 + 1)}{C} + B
        \end{gather*}
        In case $C = 0$
        \[y = \int \frac{2xdx}{0x^2 + 1} = \int 2xdx = x^2 + B\]
    \end{problem}
\end{document}