\documentclass[12pt,a4paper]{article}
\usepackage{solutions-en}
\usepackage{float}

\title{Homework of 11.27\\Differential equations and dynamic systems.\\Solutions.}
\author{Глеб Минаев @ 204 (20.Б04-мкн)}
\date{}

\renewcommand{\Re}{\mathrm{Re}}
\renewcommand{\Im}{\mathrm{Im}}
\newcommand{\sign}{\mathrm{sign}}

\begin{document}
    \maketitle

    \begin{problem}{513}
        \[y'' - 2y' = 0\]
        Characteristic poylomial $\lambda^2 - 2\lambda = 0$ has roots $0$ and $2$. Hence
        \[y = c_1 e^{0x} + c_2 e^{2x} = c_1 + c_2 e^{2x}.\]
    \end{problem}

    \begin{problem}{519}
        \[y^{(4)} - y = 0.\]
        Characteristic polynomial $\lambda^4 - 1 = 0$ has roots $1$, $-1$, $i$ and $-i$. Hence
        \[y = c_1 e^x + c_2 e^{-x} + c_3 \sin(x) + c_4 \cos(x).\]
    \end{problem}

    \begin{problem}{524}
        \[y^{(5)} - 6 y^{(4)} + 9 y^{(3)} = 0.\]
        Characteristic polynomial $\lambda^5 - 6 \lambda^4 + 9 \lambda^3 = 0$ has roots $0$, $0$, $0$, $3$ and $3$. Hence
        \[y = (c_1 + c_2 x + c_3 x^2) e^{0x} + (c_3 + c_4 x) e^{3x} = (c_1 + c_2 x + c_3 x^2) + (c_3 + c_4 x) e^{3x}.\]
    \end{problem}

    \begin{problem}{575}
        \[y'' - 2y' + y = \frac{e^x}{x}.\]
        Characteristic polynomial $\lambda^2 - 2\lambda + 1 = 0$ has roots $1$ and $1$. Hence
        \[y = C_1(x) e^x + C_2(x) x e^x,\]
        such that
        \begin{align*}
            &\left\{
                \begin{aligned}
                    &C_1' e^x + C_2' x e^x = 0\\
                    &C_1' (e^x)' + C_2' (x e^x)' = \frac{e^x}{x}
                \end{aligned}
            \right.&
            &\left\{
                \begin{aligned}
                    &C_1' e^x + C_2' x e^x = 0\\
                    &C_1' e^x + C_2' (x+1) e^x = \frac{e^x}{x}
                \end{aligned}
            \right.&
            &\left\{
                \begin{aligned}
                    &C_1' + C_2' x = 0\\
                    &C_1' + C_2' (x+1) = \frac{1}{x}
                \end{aligned}
            \right.\\
            &\left\{
                \begin{aligned}
                    &C_1' + C_2' x = 0\\
                    &C_2' = \frac{1}{x}
                \end{aligned}
            \right.&
            &\left\{
                \begin{aligned}
                    &C_1' = -1\\
                    &C_2' = \frac{1}{x}
                \end{aligned}
            \right.&
            &\left\{
                \begin{aligned}
                    &C_1 = -x + c_1\\
                    &C_2 = \ln(x) + c_2
                \end{aligned}
            \right.
        \end{align*}
        Hence
        \[y = (-x + c_1) e^x + (\ln(x) + c_2) x e^x = (x \ln(x) + (c_2 - 1) x + c_1) e^x.\]
    \end{problem}

    \begin{problem}{620}
        \[y'' + ay' + by = 0.\]
        Let $\alpha$ and $\beta$ be roots of characteristic polynomial $\lambda^2 + a\lambda + b$. We know that $e^{\alpha x} + e^{\overline{\alpha} x}$ are solutions of the equations. Then $\alpha$ must have negative real part. Because
        \[0 = \lim_{x \to + \infty} e^{\alpha x} + e^{\overline{\alpha} x} = \lim_{x \to + \infty} e^{\Re(\alpha)x} \cdot \cos(\Im(\alpha) x),\]
        hence either $\Im(\alpha) = 0$ and $\lim_{x \to +\infty} e^{\Re(\alpha)x} = 0$ means $\Re(\alpha) < 0$ or $\Im(\alpha) \neq 0$ and
        \[
            0
            = \lim_{n \to +\infty} e^{2 \pi n\Re(\alpha)/|\Im(\alpha)|} \cos(\sign(\Im(\alpha))2\pi n)
            = \lim_{n \to +\infty} e^{2 \pi n\Re(\alpha)/|\Im(\alpha)|}
        \]
        means $\Re(\alpha) < 0$. And if real parts of $\alpha$ and $\beta$ are negative then any solution $y = c_1 e^{\alpha x} + c_2 e^{\beta x} \to 0$ when $x \to + \infty$ (in case $\alpha = \beta$ $y = (c_1 + c_2x) e^{\alpha x} \to 0$ when $x \to 0$).

        But
        \begin{align*}
            &\alpha = \frac{-b + \sqrt{b^2 - 4c}}{2}&
            &\beta = \frac{-b - \sqrt{b^2 - 4c}}{2}.
        \end{align*}
        So if $b^2 - 4c < 0$, then $b = -2\Re(\alpha) = -2\Re(\beta) > 0$. And if $b^2 - 4c \geqslant 0$, then
        \[0 > \Re(\alpha) = \frac{-b + \sqrt{b^2 - 4c}}{2}\]
        that is equivalent to
        \begin{gather*}
            b > \sqrt{b^2 - 4c}\\
            b^2 > b^2 - 4c\\
            c > 0
        \end{gather*}
        (in that case if $\Re(a) < 0$, then $\Re(b) = \frac{-b - \sqrt{b^2 - 4c}}{2} < 0$).

        Hence the sought condition is
        \[
            \left\{
                \begin{aligned}
                    &b > 0\\
                    &\left[
                        \begin{aligned}
                            &c > \frac{b^2}{4}\\
                            &0 < c \leqslant \frac{b^2}{4}
                        \end{aligned}
                    \right.
                \end{aligned}
            \right.
            \quad \Longleftrightarrow \quad
            \left\{
                \begin{aligned}
                    &b > 0\\
                    &c > 0\\
                \end{aligned}
            \right.
        \]
    \end{problem}

    \begin{problem}{590}
        \[x^2 y'' - x y' - 3y = 0.\]
        Characteristic polynomial $\lambda(\lambda - 1) - \lambda - 3 = \lambda^2 - 2\lambda - 3$ has roots $-1$ and $3$. Hence
        \[y(e^t) = c_1 e^{-t} + c^2 e^{3t}.\]
    \end{problem}
\end{document}