\documentclass[12pt,a4paper]{article}
\usepackage{solutions-en}
\usepackage{float}

\title{Homework of 11.02\\Differential equations and dynamic systems.\\Solutions.}
\author{Глеб Минаев @ 204 (20.Б04-мкн)}
\date{}

\newcommand{\const}{\mathrm{const}}

\begin{document}
    \maketitle

    \begin{problem*}
        \begin{gather*}
            (1 + e^y) dx - e^{2y} \sin(x)^3 dy = 0\\
            \intertext{(lose case $\sin(x) = 0$, that is $x \equiv \pi n$ for some $n \in \ZZ$)}
            y' = \frac{dy}{dx} = \frac{1 + e^y}{e^{2y}} \frac{1}{\sin(x)^3}.
        \end{gather*}
        So there is integral
        \begin{align*}
            G
            &:= \int \frac{e^{2y}}{1 + e^y}dy - \int \frac{dx}{\sin(x)^3}\\
            &= e^y - \ln(1+e^y) - \frac{\cos(x)}{2(\cos(x)^2-1)} - \frac{1}{4} \ln\left(\frac{1-\cos(x)}{1+\cos(x)}\right) + C = 0
        \end{align*}
        So because function $f(t) = e^t - t$ is hard to inverse, $y$ cannot be expressed elementary of $x$.
    \end{problem*}

    \begin{problem*}
        \begin{gather*}
            y' = \left(\frac{y+1}{x+y-2}\right)^2
        \end{gather*}
        Let $x = u + 3$, $y = v - 1$. Then
        \begin{gather*}
            v' = \left(\frac{v}{u+v}\right)^2
        \end{gather*}
        Let $v = pu$. Then
        \begin{gather*}
            up' + p = v' = \left(\frac{1}{1+v/u}\right)^2 = \frac{1}{(1+p)^2}\\
            p' = \frac{1 - p(1+p)^2}{(1+p)^2} \frac{1}{u}.
        \end{gather*}
        So there is integral
        \begin{align*}
            G
            &:= \int \frac{(1+p)^2 dp}{1 - p(1+p)^2} - \int \frac{du}{u}\\
            &= \sum_{\alpha^3 - \alpha^2 - 1 = 0} \frac{\alpha}{3\alpha - 2} \ln(p - \alpha + 1) - \ln(u) - C = 0.
        \end{align*}
    \end{problem*}

    \begin{problem}{426}
        \begin{gather*}
            y y'' + 1 = y'^2
        \end{gather*}
        Let $p(y) = y'$. Then $y'' = pp'$, so
        \begin{gather*}
            ypp' + 1 = p^2\\
            p' = \frac{p^2 - 1}{p} \frac{1}{y}
        \end{gather*}
        If $\frac{p^2 - 1}{p} = 0$, then $p^2 = 1$, so $p = \pm 1$, $y = C \pm x$. Otherwise there is integral
        \begin{align*}
            G
            &:= \int \frac{pdp}{p^2 - 1} - \int \frac{dy}{y}\\
            &= \frac{1}{2}\ln(p^2 - 1) - \ln(y) + C = 0
        \end{align*}
        Hence
        \begin{gather*}
            \ln(p^2 - 1) = C + 2\ln(y)\\
            p^2 - 1 = C y^2\\
            y' = p = \pm \sqrt{1 + Cy^2}.
        \end{gather*}
        If $\pm \sqrt{1 + Cy^2} = 0$, then $y = \pm 1/\sqrt{-C}$. Otherwise there is integral
        \begin{align*}
            H
            &:= \int \frac{dy}{\pm \sqrt{1 + Cy^2}} - \int dx\\
            &= \pm \frac{\sinh^{-1}(\sqrt{C}y)}{\sqrt{C}} - x + D = 0.
        \end{align*}
        Hence
        \begin{gather*}
            y = \pm \frac{\sinh(\sqrt{C}x + \sqrt{C} D)}{\sqrt{C}} = \pm \frac{\sinh(ax + b)}{a}.
        \end{gather*}
    \end{problem}

    \begin{problem}{446}
        \begin{gather*}
            (y' + 2y)y'' = y'^2
        \end{gather*}
        Let $p(y) = y'$. Then $y'' = pp'$, so
        \begin{gather*}
            (p + 2y)pp' = p^2
            \intertext{(lose case $p \equiv 0$, where $y \equiv \const$)}
            p' = \frac{p}{p + 2y}
        \end{gather*}
        Let $p = qy$. Then
        \begin{gather*}
            yq' + q = \frac{q}{q + 2}\\
            q' = \frac{-q(q+1)}{q+2} \frac{1}{y}
        \end{gather*}
        If $\frac{-q(q+1)}{q+2}=0$, then $q \in \{0; -1\}$, $p = 0$ or $p = -y$, $y \equiv \const$ or $y = Ce^{-x}$. Otherwise there is integral
        \begin{align*}
            G
            &:= \int -\frac{q+2}{q(q+1)} dq - \int \frac{dy}{y}\\
            &= \int \left(\frac{1}{q+1} - \frac{2}{q}\right) dq - \ln(y)\\
            &= \ln(q+1) - 2\ln(q) - \ln(y) + C = 0
        \end{align*}
        Hence
        \begin{gather*}
            \ln\left(\frac{q+1}{q^2}\right) = \ln(Cy)\\
            \frac{q+1}{q^2} = Cy\\
            q = \frac{1 \pm \sqrt{1 + 4Cy}}{2Cy}\\
            y' = p = qy = \frac{1 \pm \sqrt{1 + 4Cy}}{2C}
        \end{gather*}
        So there is integral
        \begin{align*}
            H
            &:= \int \frac{2Cy}{1 \pm \sqrt{1 + 4Cy}} dy - \int dx\\
            &= \pm \sqrt{1 + 4Cy} - \ln(1 \pm \sqrt{1 + 4Cy}) - x + D = 0
        \end{align*}
    \end{problem}
\end{document}